src/NodeSt.v
@@ -1,0 +1,43 @@
+Require Import Term_Defs ConcreteEvidence.
+
+Require Import StructTact.Update.
+
+Inductive Prim_Instr: Set :=
+| copy: Prim_Instr
+| umeas: ASP_ID -> list Arg -> Prim_Instr
+| sign: Prim_Instr
+| hash: Prim_Instr.
+
+Inductive AnnoInstr: Set :=
+| aprimInstr: nat -> Prim_Instr -> AnnoInstr
+| aReq: nat -> nat -> VM_ID -> AnnoInstr
+| aseq: AnnoInstr -> AnnoInstr -> AnnoInstr.
+
+Definition asp_instr (a:ASP) : Prim_Instr :=
+  match a with
+  | CPY => copy
+  | ASPC i args => umeas i args
+  | SIG => sign
+  | HSH => hash
+  end.
+
+Fixpoint instr_compiler (t:AnnoTerm) : AnnoInstr :=
+  match t with
+  | aasp (i,_) a => aprimInstr i (asp_instr a)
+  | aatt (i,j) p q _ =>
+    (aReq i (Nat.pred j) q)
+  | alseq _ t1 t2 => aseq (instr_compiler t1) (instr_compiler t2)
+  end.
+
+Definition tr_asp_instr (x:nat) (p:Plc) (pi:Prim_Instr) :=
+  match pi with
+  | copy => Term_Defs.copy x p
+  | umeas asp_id args => (Term_Defs.umeas x p asp_id args)
+  | sign => Term_Defs.sign x p
+  | hash => Term_Defs.hash x p
+  end.
+
+
+
+
+
