src/NodeTest.v
@@ -1,0 +1,121 @@
+Require Import Coq.Arith.PeanoNat.
+Require Import Coq.Logic.ProofIrrelevance Coq.Program.Equality.
+
+Require Import List.
+Import ListNotations.
+
+Require Import Lia.
+
+(*
+Require Import StructTact.StructTactics.
+*)
+
+Set Nested Proofs Allowed.
+
+Section NodeTest.
+
+  Variable num_Servers : nat.
+
+  Definition Server_index := {n:nat | n < num_Servers}.
+
+  Definition Name := Server_index.
+
+  
+  Definition Name_eq_dec : forall a b : Name, {a = b} + {a <> b}.
+    intros.
+    unfold Name in *.
+    destruct a; destruct b.
+    destruct (Nat.eq_dec x x0).
+    -
+      subst.
+      assert (l = l0).
+      {
+        eapply proof_irrelevance.
+      }
+      subst.
+      left.
+      reflexivity.
+    -
+      subst.
+      right.
+      unfold not.
+      intros.
+      inversion H.
+      congruence.
+  Defined.
+
+  (* TODO:  I want the equivalent of:  [0; 1; ... (num_Servers - 1)], 
+     but instead a list of dependent pairs, each with an element and a
+     proof saying that "element is less than num_Servers". *)
+
+
+
+(*
+  Definition sumbool_wrap_nat (n:nat):  (n < num_Servers) + (n >= num_Servers).
+  Admitted.
+
+  Definition wrap_nat (n:nat): (n < num_Servers).
+  Admitted.
+*)
+
+  Definition list_Servers_dep : {l:list Name | map (@proj1_sig _ _) l = (seq 0 num_Servers)}.
+  Admitted.
+
+  Definition list_Servers : list Name := proj1_sig list_Servers_dep.
+
+
+  Definition Nodes := list_Servers.
+
+  Lemma seq_fact: forall n n',
+    S n < S n' ->
+    In (S n) (seq 1 n').
+  Proof.
+  Admitted.
+  
+
+  Theorem In_n_Nodes :
+    forall n : Name, In n Nodes.
+  Proof using.
+    intros.
+    unfold Nodes, list_Servers.
+    destruct list_Servers_dep.
+    unfold Name in *.
+    unfold Server_index in *. 
+    simpl.
+    destruct n.
+
+    assert (In x0 (seq 0 num_Servers)).
+    {
+      destruct num_Servers;
+        destruct x0;
+        try lia.
+      +
+        simpl.
+        eauto.
+      +
+        simpl.
+        right.
+        eapply seq_fact; eauto.
+    }
+  (* NOW WHAT?? *)
+  Abort.
+
+  Theorem nodup :
+    NoDup Nodes.
+  Proof using.
+    unfold Nodes, list_Servers.
+    destruct list_Servers_dep.
+    simpl.
+    unfold Name in *.
+    unfold Server_index in *.
+
+    assert (NoDup (seq 0 num_Servers)).
+    {
+      eapply seq_NoDup.
+    }
+  (* NOW WHAT?? *)
+  Abort.
+
+
+
+End NodeTest.
