src/Seq_Facts.v
@@ -1,0 +1,69 @@
+Require Import List.
+Import ListNotations.
+
+Require Import Lia.
+
+Require Import StructTact.StructTactics.
+
+Lemma seq_nonzero_fact: forall n n',
+    n > 0 -> 
+    In 0 (seq n n') ->
+    False.
+Proof.
+Admitted.
+
+Lemma seq_fact' : forall n n',
+    In n (seq 1 n') ->
+    In (S n) (seq 2 n').
+Proof.
+  intros.
+    generalizeEverythingElse n.
+    induction n; destruct n'; intros;
+      try solve_by_inversion.
+    -
+      simpl in *.
+      destruct H;
+        try solve_by_inversion.
+
+      exfalso.
+      eapply seq_nonzero_fact with (n:=2) (n':=n').
+      lia.
+      eassumption.
+    -
+      simpl in *.
+      destruct H;
+        try solve_by_inversion.
+
+      destruct n.
+      +
+        left.
+        tauto.
+      +
+        right.
+
+        assert (2 <= (S (S n)) < 2 + n').
+        {
+          eapply in_seq.
+          eassumption.
+        }
+Admitted.
+
+Lemma seq_fact: forall n n',
+    S n < S n' ->
+    In (S n) (seq 1 n').
+Proof.
+  intros.
+  generalizeEverythingElse n'.
+  induction n'; destruct n; intros;
+    try lia;
+    try (simpl; eauto; tauto).
+  -
+    simpl.
+    right.
+    pose (IHn' n).
+
+    assert (S n < S n') by lia.
+    pose (i H0).
+
+    eapply seq_fact'; eauto.
+Defined.
